most of tseytin correctness proof, OR case is wip

theories/L/Complexity/Cook/FSAT_to_SAT.v
@@ -4,6 +4,53 @@ From Undecidability.L.Complexity.Cook Require Import Prelim FSAT SAT.
 From Undecidability.L.Datatypes Require Import LLists. 
 Require Import Lia. 
 
+Definition varInLiteral v (l : literal) := exists b, l = (b, v).
+Definition varInClause v c := exists l, l el c /\ varInLiteral v l. 
+Definition varInCnf v cn := exists cl, cl el cn /\ varInClause v cl. 
+
+
+Definition clause_varsIn (p : nat -> Prop) c := forall v, varInClause v c -> p v. 
+Definition cnf_varsIn (p : nat -> Prop) c := forall v, varInCnf v c -> p v. 
+
+Lemma clause_varsIn_varBound c n : clause_varsIn (fun v => v < n) c <-> varBound_clause n c. 
+Proof. 
+  induction c. 
+  - split; intros H; [eauto | intros v (? & [] &_)].
+  - split; intros H.
+    + destruct a as (b & v). econstructor.
+      * apply (H v). exists (b, v). split; [now left | exists b; easy].
+      * apply IHc. intros v' (l & H1). apply H. exists l. easy.
+    + inv H. apply IHc in H3. intros v (l & [<- | H4] & H5). 
+      * destruct H5 as (b' & H5). inv H5. lia. 
+      * apply H3. exists l. easy.
+Qed.
+
+Lemma cnf_varsIn_varBound c n: cnf_varsIn (fun v => v < n) c <-> varBound_cnf n c. 
+Proof. 
+  induction c. 
+  - split; intros H; [eauto | intros v (? & [] & _) ]. 
+  - split; intros H. 
+    + econstructor.
+      * apply clause_varsIn_varBound. intros v H1. apply H. exists a. easy. 
+      * apply IHc. intros v' (cl & H1). apply H. exists cl. easy.
+    + inv H. apply IHc in H3. apply clause_varsIn_varBound in H2. intros v (cl & [<- | H4] & H5). 
+      * apply (H2 v H5). 
+      * apply H3. exists cl. easy.
+Qed.
+
+Lemma cnf_varsIn_app c1 c2 p : cnf_varsIn p (c1 ++ c2) <-> cnf_varsIn p c1 /\ cnf_varsIn p c2. 
+Proof. 
+  unfold cnf_varsIn. unfold varInCnf. setoid_rewrite in_app_iff. split; [intros H  |intros [H1 H2]].
+  - split; intros v [cl [H3 H4]]; apply H; eauto.
+  - intros v [cl [[H3 | H3] H4]]; [apply H1 | apply H2]; eauto.
+Qed.
+
+Lemma cnf_varsIn_monotonic (p1 p2 : nat -> Prop) c : (forall n, p1 n -> p2 n) -> cnf_varsIn p1 c -> cnf_varsIn p2 c. 
+Proof. 
+  intros H H1 v H2. apply H, H1, H2. 
+Qed. 
+
+
 (*v <-> (v1 ∧ v2) *)
 Definition tseytinAnd (v v1 v2 : var) : cnf := 
 [[(false, v); (true, v1)]; [(false, v); (true, v2)]; [(false, v1); (false, v2); (true, v)]].
@@ -13,6 +60,8 @@ Definition tseytinOr (v v1 v2 : var) : cnf :=
 (* v <-> ¬ v'*)
 Definition tseytinNot (v v' : var) : cnf := 
   [[(false, v); (false, v')]; [(true, v); (true, v')]].
+Definition tseytinEquiv (v v' : var) : cnf := 
+  [[(false, v); (true, v')]; [(false, v'); (true, v)]]. 
 
 Lemma tseytinAnd_sat a v v1 v2 : satisfies a (tseytinAnd v v1 v2) <-> (evalVar a v = true <-> (evalVar a v1 = true /\ evalVar a v2 = true)). 
 Proof. 
@@ -36,37 +85,46 @@ Proof.
   (split; [intros H; try congruence; split; intros; congruence | tauto]).
 Qed.
 
-Lemma tseytinAnd_varBound v v1 v2 : varBound_cnf (S (Nat.max v (Nat.max v1 v2))) (tseytinAnd v v1 v2). 
+Lemma tseytinEquiv_sat a v v' : satisfies a (tseytinEquiv v v') <-> (evalVar a v = true <-> evalVar a v' = true). 
 Proof. 
-  unfold tseytinAnd. repeat match goal with 
-    | [ |- varBound_clause _ _] => constructor 
-    | [ |- varBound_cnf _ _ ] => constructor
-    | _ => lia
-  end. 
+  unfold tseytinEquiv, satisfies. 
+  destruct (evalVar a v) eqn:H1, (evalVar a v') eqn:H2; cbn in *; 
+    repeat (first [rewrite H1 | rewrite H2]; cbn); tauto.
+Qed.
+
+Ltac cnf_varsIn_force := 
+  match goal with [ |- cnf_varsIn _ _ ] => 
+      let v := fresh "v" in let H1 := fresh "H1" in let H2 := fresh "H2" in let H3 := fresh "H3" in  
+      intros v [? [H1 H2]]; cbn in H1; destruct_or H1; inv H1; 
+      destruct H2 as [? [H2 H3]]; cbn in H2; destruct_or H2; inv H2; 
+      destruct H3 as [? H3]; inv H3; eauto
+  end.
+
+Lemma tseytinAnd_cnf_varsIn v v1 v2 : cnf_varsIn (fun n => n = v \/ n= v1 \/ n = v2) (tseytinAnd v v1 v2). 
+Proof. 
+  unfold tseytinAnd. cnf_varsIn_force.
+Qed.
+
+Lemma tseytinOr_cnf_varsIn v v1 v2 : cnf_varsIn (fun n => n = v \/ n = v1 \/ n = v2) (tseytinOr v v1 v2).
+Proof. 
+  unfold tseytinOr. cnf_varsIn_force. 
 Qed. 
 
-Lemma tseytinOr_varBound v v1 v2 : varBound_cnf (S (Nat.max v (Nat.max v1 v2))) (tseytinOr v v1 v2). 
+Lemma tseytinNot_cnf_varsIn v v' : cnf_varsIn (fun n => n = v \/ n = v') (tseytinNot v v'). 
 Proof. 
-  unfold tseytinOr. repeat match goal with 
-    | [ |- varBound_clause _ _] => constructor 
-    | [ |- varBound_cnf _ _ ] => constructor
-    | _ => lia
-  end. 
+  unfold tseytinNot. cnf_varsIn_force. 
 Qed. 
 
-Lemma tseytinNot_varBound v v' : varBound_cnf (S (Nat.max v v')) (tseytinNot v v'). 
+Lemma tseytinEquiv_cnf_varsIn v v' : cnf_varsIn (fun n => n = v \/ n = v') (tseytinEquiv v v').
 Proof. 
-  unfold tseytinNot. repeat match goal with 
-    | [ |- varBound_clause _ _] => constructor 
-    | [ |- varBound_cnf _ _ ] => constructor
-    | _ => lia
-  end. 
-Qed. 
+  unfold tseytinEquiv. cnf_varsIn_force.
+Qed.
+
 
 Fixpoint tseytin' (nfVar : var) (f : formula) : (var * cnf * var) := 
   match f with 
   | Ftrue => (nfVar, [[(true, nfVar)]], S nfVar)
-  | Fvar v => (v, [], nfVar)
+  | Fvar v => (nfVar, tseytinEquiv v nfVar, S nfVar) (*in principle, we could directly return v; however, using a fresh variable makes the proof easier *)
   | For f1 f2 => let
       '(rv1, N1, nfVar1) := tseytin' nfVar f1 in let 
       '(rv2, N2, nfVar2) := tseytin' nfVar1 f2 in 
@@ -102,24 +160,29 @@ Hint Resolve varBound_cnf_app.
 Hint Constructors varBound_cnf varBound_clause. 
 
 (*for the proof of correctness, a stronger notion of representation is needed *)
-Definition assignment_lower_bound a n := forall v, v el a -> v >= n.
+Definition assgn_varsIn (p : nat -> Prop) a := forall v, v el a -> p v. 
 Definition restrict a n := filter (fun v => v <? n) a.
 Definition join (a a' : assgn) := a ++ a'.
 
-Lemma assignment_lower_bound_app a1 a2 n: assignment_lower_bound (a1 ++ a2) n <-> assignment_lower_bound a1 n /\ assignment_lower_bound a2 n.
+Lemma assgn_varsIn_app p a1 a2 : assgn_varsIn p (a1 ++ a2) <-> assgn_varsIn p a1 /\ assgn_varsIn p a2. 
 Proof. 
-  unfold assignment_lower_bound. setoid_rewrite in_app_iff. firstorder.
+  unfold assgn_varsIn. setoid_rewrite in_app_iff. firstorder.
 Qed.
 
-Lemma assignment_lower_bound_monotonic a n n' : assignment_lower_bound a n -> n >= n' -> assignment_lower_bound a n'. 
-Proof. 
-  intros H H1. unfold assignment_lower_bound in *. intros v Hv; specialize (H v Hv); lia. 
-Qed. 
+Lemma assgn_varsIn_monotonic (p1 p2 : nat -> Prop) a : (forall n, p1 n -> p2 n) -> assgn_varsIn p1 a -> assgn_varsIn p2 a.
+Proof. intros H H1 v H0. eauto. Qed. 
 
 Lemma evalVar_monotonic a a' v : a <<= a' -> evalVar a v = true -> evalVar a' v = true.
 Proof. 
   intros H1 H2. rewrite evalVar_in_iff in *. firstorder.
 Qed. 
+
+Lemma evalVar_assgn_equiv a a' v : a === a' -> evalVar a v = evalVar a' v. 
+Proof. 
+  intros H. enough (evalVar a v = true <-> evalVar a' v = true).
+  { destruct evalVar, evalVar; firstorder. }
+  split; apply evalVar_monotonic; apply H. 
+Qed.
 
 Lemma evalLiteral_assgn_equiv a1 a2 l : a1 === a2 -> evalLiteral a1 l = evalLiteral a2 l. 
 Proof. 
@@ -142,70 +205,6 @@ Proof.
   - destruct evalCnf; destruct evalCnf; firstorder; easy.
   - rewrite !evalCnf_clause_iff. now setoid_rewrite (evalClause_assgn_equiv _ H).
 Qed. 
-
-Definition varInLiteral v (l : literal) := exists b, l = (b, v).
-Definition varInClause v c := exists l, l el c /\ varInLiteral v l. 
-Definition varInCnf v cn := exists cl, cl el cn /\ varInClause v cl. 
-
-
-Definition clause_varsIn (p : nat -> Prop) c := forall v, varInClause v c -> p v. 
-Definition cnf_varsIn (p : nat -> Prop) c := forall v, varInCnf v c -> p v. 
-
-Lemma clause_varsIn_varBound c n : clause_varsIn (fun v => v < n) c <-> varBound_clause n c. 
-Proof. 
-  induction c. 
-  - split; intros H; [eauto | intros v (? & [] &_)].
-  - split; intros H.
-    + destruct a as (b & v). econstructor.
-      * apply (H v). exists (b, v). split; [now left | exists b; easy].
-      * apply IHc. intros v' (l & H1). apply H. exists l. easy.
-    + inv H. apply IHc in H3. intros v (l & [<- | H4] & H5). 
-      * destruct H5 as (b' & H5). inv H5. lia. 
-      * apply H3. exists l. easy.
-Qed.
-
-Lemma cnf_varsIn_varBound c n: cnf_varsIn (fun v => v < n) c <-> varBound_cnf n c. 
-Proof. 
-  induction c. 
-  - split; intros H; [eauto | intros v (? & [] & _) ]. 
-  - split; intros H. 
-    + econstructor.
-      * apply clause_varsIn_varBound. intros v H1. apply H. exists a. easy. 
-      * apply IHc. intros v' (cl & H1). apply H. exists cl. easy.
-    + inv H. apply IHc in H3. apply clause_varsIn_varBound in H2. intros v (cl & [<- | H4] & H5). 
-      * apply (H2 v H5). 
-      * apply H3. exists cl. easy.
-Qed.
-
-(*it does not suffice to use formula_maxVar f instead of the parameter bound: the induction will fail 
-  as we have to show that formula_maxVar (f1 ∧ f2) is a lower bound...*)
-Definition tseytin_formula_repr (f : formula) (N : cnf) (v : var) (bound : nat):= 
-  (forall a, FSAT.satisfies a f -> exists a', assignment_lower_bound a' bound /\ SAT.satisfies (join a' a) ([(true, v)] :: N))
-  /\ (forall a, SAT.satisfies a ([(true, v)] :: N) -> FSAT.satisfies (restrict a (formula_maxVar f)) f). 
-
-Lemma join_extension_formula_equisat n f a a': varBound_formula n f -> assignment_lower_bound a' n -> (FSAT.satisfies a f <-> FSAT.satisfies (join a a') f).
-Proof. 
-  intros H H0.
-  unfold FSAT.satisfies. induction f. 
-  - cbn; tauto.
-  - rewrite !evalFormula_prim_iff. inv H. unfold assignment_lower_bound in H0.
-    unfold join.
-    split; [intros; now apply in_app_iff | ]. 
-    intros [H1 | H1]%in_app_iff; [easy | ].
-    apply H0 in H1. lia.  
-  - inv H. rewrite !evalFormula_and_iff. 
-    apply (varBound_formula_monotonic H5) in H3. 
-    apply (varBound_formula_monotonic H6) in H4.
-    apply IHf1 in H3. apply IHf2 in H4. 
-    tauto.
-  - inv H. rewrite !evalFormula_or_iff. 
-    apply (varBound_formula_monotonic H5) in H3. 
-    apply (varBound_formula_monotonic H6) in H4.
-    apply IHf1 in H3. apply IHf2 in H4. 
-    tauto.
-  - inv H. apply IHf in H2. rewrite !evalFormula_not_iff. tauto.
-Qed.
-
 
 (*an actually usable version of the lemma without useless bool2Prop stuff *)
 Lemma in_filter_iff (X : Type) (x : X) (p : X -> bool) (A : list X): x el filter p A <-> x el A /\ p x = true. 
@@ -238,141 +237,425 @@ Qed.
 Fact app_singleton (X : Type) (x : X) (l : list X) : x::l = [x] ++ l. 
 Proof. easy. Qed.
 
-Lemma join_extension_cnf_monotonic a a' c : SAT.satisfies a c -> SAT.satisfies (join a' a) c. 
+Lemma evalVar_not_assgn_varsIn_false p a v : assgn_varsIn p a -> (not (p v)) -> evalVar a v = false. 
 Proof. 
-  (*intros H. unfold join. apply *)
-Admitted. 
+  intros H H1. 
+  destruct evalVar eqn:H2; [ | easy]. exfalso; apply H1.
+  apply evalVar_in_iff in H2. now apply H in H2. 
+Qed.
+
+Lemma join_extension_var_sat a a' (p1 p2 : nat -> Prop) v : p1 v -> assgn_varsIn p2 a' -> (forall n, not (p1 n /\ p2 n)) -> evalVar a v = evalVar (join a' a) v.
+Proof. 
+  intros H1 H2 H3. 
+  enough (evalVar a v = true <-> evalVar (join a' a) v = true). 
+  { destruct (evalVar a v), (evalVar (join a' a) v); cbn in *; firstorder. }
+  unfold evalVar. rewrite !list_in_decb_iff. 2,3: symmetry; apply Nat.eqb_eq.
+  unfold assgn_varsIn in H2. unfold join.
+  split; [ eauto | intros [H4 | H4]%in_app_iff]; [ | easy].
+  apply H2 in H4. exfalso; apply (H3 v); tauto.
+Qed.
+
+Lemma join_extension_literal_sat a a' (p1 p2 : nat -> Prop) b v : p1 v -> assgn_varsIn p2 a' -> (forall n, not (p1 n /\ p2 n)) -> evalLiteral a (b, v) = true <-> evalLiteral (join a' a) (b, v) = true. 
+Proof. 
+  intros H1 H2 H3. unfold evalLiteral. rewrite !eqb_true_iff. 
+  enough (evalVar a v = evalVar (join a' a) v) as H by (rewrite H; tauto). 
+  now eapply join_extension_var_sat.
+Qed. 
+
+Lemma join_extension_clause_sat a a' p1 p2 c : clause_varsIn p1 c -> assgn_varsIn p2 a' -> (forall n, not (p1 n /\ p2 n)) -> evalClause a c = true <-> evalClause (join a' a) c = true.
+Proof. 
+  intros H1 H2 H3. 
+  rewrite !evalClause_literal_iff. split; intros [l [F1 F2]]; exists l. 
+  - split; [apply F1 | ]. destruct l as (b & v). erewrite <- join_extension_literal_sat; try easy. 
+    apply H1. exists (b, v). split; [apply F1 | exists b; easy].
+  - split; [apply F1 | ]. destruct l as (b & v). erewrite join_extension_literal_sat; try easy. 
+    apply H1. exists (b, v). split; [apply F1 | exists b; easy].
+Qed.
+
+Lemma join_extension_cnf_sat a a' p1 p2 c: cnf_varsIn p1 c -> assgn_varsIn p2 a' -> (forall n, not (p1 n /\ p2 n)) -> evalCnf a c = true <-> evalCnf (join a' a) c = true. 
+Proof. 
+  intros H1 H2 H3. rewrite !evalCnf_clause_iff. split; intros H cl F1; specialize (H cl F1).
+  - erewrite <- join_extension_clause_sat; try easy. intros v F2. eapply H1. exists cl; eauto.
+  - erewrite join_extension_clause_sat; try easy. intros v F2. eapply H1. exists cl; eauto.
+Qed. 
+
+Ltac list_equiv := let x := fresh "x" in let Hx := fresh "Hx" in 
+  try rewrite <- !app_assoc;
+  split; intros x; rewrite !in_app_iff; intros Hx; destruct_or Hx; eauto.
+
+(*it does not suffice to use formula_maxVar f instead of the parameter bound: the induction will fail 
+  as we have to show that formula_maxVar (f1 ∧ f2) is a lower bound...*)
+Definition tseytin_formula_repr (f : formula) (N : cnf) (v : var) (b nf nf' : nat):= 
+  (forall a, assgn_varsIn (fun n => n < b) a -> exists a', assgn_varsIn (fun n => n >= nf /\ n < nf') a' /\ SAT.satisfies (join a' a) N /\ (FSAT.satisfies a f <-> evalVar (join a' a) v = true))
+  /\ (forall a, SAT.satisfies a N -> (evalVar a v = true <-> FSAT.satisfies (restrict a b) f)). 
+
+Lemma evalFormula_and_iff' f1 f2 a: evalFormula a (f1 ∧ f2) = false <-> evalFormula a f1 = false \/ evalFormula a f2 = false. 
+Proof. 
+  cbn.  destruct (evalFormula a f1), (evalFormula a f2); cbn; tauto.
+Qed. 
 
 Lemma and_compat f1 f2 b: 
   varBound_formula b f1 -> varBound_formula b f2 
-  -> (forall nf nf' v N, nf >= b -> tseytin' nf f1 = (v, N, nf') -> cnf_varsIn (fun n => n < b \/ (n >= nf /\ n < nf')) N /\ v < nf' /\ tseytin_formula_repr f1 N v nf)
-  -> (forall nf nf' v N, nf >= b -> tseytin' nf f2 = (v, N, nf') -> cnf_varsIn (fun n => n < b \/ (n >= nf /\ n < nf')) N /\ v < nf' /\ tseytin_formula_repr f2 N v nf)
-  -> forall nf nf' v N, nf >= b -> tseytin' nf (f1 ∧ f2) = (v, N, nf') -> cnf_varsIn (fun n => n < b \/ (n >= nf /\ n < nf')) N /\ v < nf' /\ tseytin_formula_repr (f1 ∧ f2) N v nf. 
+  -> (forall nf nf' v N, nf >= b -> tseytin' nf f1 = (v, N, nf') -> cnf_varsIn (fun n => n < b \/ (n >= nf /\ n < nf')) N /\ v >= nf /\ v < nf' /\ tseytin_formula_repr f1 N v b nf nf')
+  -> (forall nf nf' v N, nf >= b -> tseytin' nf f2 = (v, N, nf') -> cnf_varsIn (fun n => n < b \/ (n >= nf /\ n < nf')) N /\ v >= nf /\ v < nf' /\ tseytin_formula_repr f2 N v b nf nf')
+  -> forall nf nf' v N, nf >= b -> tseytin' nf (f1 ∧ f2) = (v, N, nf') -> cnf_varsIn (fun n => n < b \/ (n >= nf /\ n < nf')) N /\ v >= nf /\ v < nf' /\ tseytin_formula_repr (f1 ∧ f2) N v b nf nf'. 
 Proof. 
-  (*cbn. intros IHf1 IHf2 nf nf' v N H H0.*)
-  (*destruct (tseytin' nf f1) as ((rv1 & N1) & nfVar1) eqn:F1.*)
-  (*destruct (tseytin' nfVar1 f2) as ((rv2 & N2) & nfVar2) eqn:F2. *)
-  (*inv H. *)
-  (*specialize (@varBound_formula_monotonic f1 n1 nf ltac:(lia) H3) as H3'.*)
-  (*specialize (tseytin'_nf_monotonic F1) as H7. *)
-  (*specialize (tseytin'_nf_monotonic F2) as H8.*)
-  (*specialize (@varBound_formula_monotonic f2 n2 nfVar1 ltac:(lia) H4) as H4'.*)
-  (*specialize (IHf1 nf nfVar1 _ _  H3' F1) as (IH1 & IH3 & IH2 & (IH31 & IH32)).*)
-  (*specialize (IHf2 nfVar1 nfVar2 _ _ H4' F2) as (IH4 & IH6 & IH5 & (IH61 & IH62)).*)
-  (*symmetry in H0. inv H0. split; [ | split; [ | split; [lia | ]]].*)
-  (*- apply varBound_cnf_app; split; [ | apply varBound_cnf_app; split]; eauto 9.*)
-    (*eapply varBound_cnf_monotonic. 2: apply tseytinAnd_varBound. lia.*)
-  (*-  *)
-  (*- split; intros a H.*)
-    (*+ clear IH62 IH32. unfold FSAT.satisfies in H. apply evalFormula_and_iff in H as (He1 & He2).*)
-      (*specialize (IH31 _ He1) as (a1' & G1 & G2). *)
-      (*specialize (IH61 _ He2) as (a2' & G3 & G4).*)
-      (*exists (nfVar2 :: a2' ++ a1'). split.*)
-      (*1: { *)
-        (*replace (nfVar2 :: a2' ++a1') with ([nfVar2] ++ a2' ++ a1') by easy. rewrite !assignment_lower_bound_app. *)
-        (*repeat split; [ | eapply assignment_lower_bound_monotonic; [apply G3 | lia] | easy]. intros v' [<- | []]. lia.*)
+  cbn. intros bound1 bound2 IHf1 IHf2 nf nf' v N H H0. 
+  destruct (tseytin' nf f1) as ((rv1 & N1) & nfVar1) eqn:F1. 
+  destruct (tseytin' nfVar1 f2) as ((rv2 & N2) & nfVar2) eqn:F2. 
+  specialize (IHf1 nf nfVar1 _ _ ltac:(lia) F1) as (IH1 & IH2 & IH2' & (IH31 & IH32)). 
+  specialize (tseytin'_nf_monotonic F1) as H7. 
+  specialize (tseytin'_nf_monotonic F2) as H8.
+  specialize (IHf2 nfVar1 nfVar2 _ _ ltac:(lia) F2) as (IH4 & IH5 & IH5' & (IH61 & IH62)). clear F1 F2.
+  symmetry in H0. inv H0. split; [ | split; [lia | split; [lia | split; [ | split]]]]. 
+  - repeat rewrite cnf_varsIn_app. 
+    repeat split.
+    + eapply cnf_varsIn_monotonic, IH1; cbn; intros. lia. 
+    + eapply cnf_varsIn_monotonic, IH4; cbn; intros; lia. 
+    + eapply cnf_varsIn_monotonic, tseytinAnd_cnf_varsIn; cbn; intros; lia.
+  - clear IH62 IH32. intros a H0'. 
+    specialize (IH31 a H0') as (a1' & G1 & G2 & G3). 
+    specialize (IH61 a H0') as (a2' & K1 & K2 & K3). 
+    (*CA : FSAT.satisfies a (f1 ∧ f2) *)
+    destruct (evalFormula a (f1 ∧ f2)) eqn:H0.
+    + specialize (proj1 (evalFormula_and_iff _ _ _) H0) as (He1 & He2).
+      apply G3 in He1. apply K3 in He2. clear G3 K3.
+      exists ([nfVar2] ++ a2' ++ a1'). split; [ | split].
+      * rewrite !assgn_varsIn_app. split; [ | split].
+        -- intros v [-> | []]; cbn; lia.
+        -- eapply assgn_varsIn_monotonic, K1. cbn; intros; lia.
+        -- eapply assgn_varsIn_monotonic, G1. cbn; intros; lia.
+      * unfold join, satisfies. rewrite !evalCnf_app_iff. repeat split.
+        -- replace (([nfVar2] ++ a2' ++ a1') ++ a) with (join (join [nfVar2] a2') (join a1' a)) by (unfold join; firstorder). 
+           erewrite <- join_extension_cnf_sat with (p2 := fun n => n = nfVar2 \/ (n >= nfVar1 /\ n < nfVar2)). 
+           ++ apply G2. 
+           ++ apply IH1.
+           ++ apply assgn_varsIn_app. split; [intros v' [-> | []]; cbn; lia | ]. 
+              eapply assgn_varsIn_monotonic, K1. cbn; intros; lia.
+           ++ cbn; intros; lia.
+        -- enough (evalCnf (join (join [nfVar2] a1') (join a2' a)) N2 = true) as He.
+           { rewrite <- He. apply evalCnf_assgn_equiv. unfold join; list_equiv. } 
+           erewrite <- join_extension_cnf_sat with (p2 := fun n => n = nfVar2 \/ (n >= nf /\ n < nfVar1)). 
+           ++ apply K2. 
+           ++ apply IH4.
+           ++ apply assgn_varsIn_app. split; [intros v' [-> | []]; cbn; lia | ].
+              eapply assgn_varsIn_monotonic, G1. cbn; intros; lia.
+           ++ cbn; intros; lia. 
+        -- apply tseytinAnd_sat. split; [intros _ | intros _; cbn; now rewrite Nat.eqb_refl]. 
+           split; eapply evalVar_monotonic.
+           2: apply He1. 3: apply He2. 
+           all: unfold join; rewrite <- app_assoc, app_singleton; intros x; rewrite !in_app_iff; intros Hx; destruct_or Hx; eauto.
+      * split; [intros _; cbn; now rewrite Nat.eqb_refl | intros _; apply H0].
+    + specialize (proj1 (evalFormula_and_iff' _ _ _) H0) as [He | He].
+      * (*first formula is false  *)
+        assert (evalVar (join a1' a) rv1 = false) as He'. 
+        { destruct (evalVar (join a1' a) rv1); [ | easy]. unfold FSAT.satisfies in G3. rewrite He in G3; firstorder. }
+        exists (a2' ++ a1'). split; [ | split].
+        -- rewrite !assgn_varsIn_app. split.
+           ++ eapply assgn_varsIn_monotonic, K1. cbn; intros; lia.
+           ++ eapply assgn_varsIn_monotonic, G1. cbn; intros; lia.
+        -- unfold join, satisfies. rewrite !evalCnf_app_iff. repeat split.
+           ++ rewrite <-app_assoc.  
+             erewrite <- join_extension_cnf_sat; [apply G2 | apply IH1 | apply K1 | cbn; intros; lia]. 
+           ++ enough (evalCnf (join a1' (join a2' a)) N2 = true) as Hee.
+             { rewrite <- Hee. apply evalCnf_assgn_equiv. unfold join; list_equiv. } 
+             erewrite <- join_extension_cnf_sat; [apply K2 | apply IH4 | apply G1 | cbn; intros; lia].
+           ++ apply tseytinAnd_sat. 
+              erewrite evalVar_not_assgn_varsIn_false with (p := fun n => n < b \/ (n >= nf /\ n < nfVar2)). 
+              2: { rewrite <- app_assoc, !assgn_varsIn_app. split; [ | split]. 
+                  - eapply assgn_varsIn_monotonic, K1. cbn; intros; lia.
+                  - eapply assgn_varsIn_monotonic, G1. cbn; intros; lia.
+                  - eapply assgn_varsIn_monotonic, H0'. cbn; intros; lia.
+              } 
+              2: lia. 
+              rewrite <- !app_assoc. erewrite <- join_extension_var_sat with (p1 := fun n => n = rv1).
+              ** unfold join in He'. rewrite He'. firstorder.
+              ** reflexivity.
+              ** apply K1. 
+              ** cbn; intros; lia.
+       -- unfold FSAT.satisfies. rewrite H0. rewrite evalVar_not_assgn_varsIn_false with (p := fun n => n < b \/ (n >= nf /\ n < nfVar2)); [easy | | ].  
+          ++ unfold join. rewrite !assgn_varsIn_app. split; [ split| ].
+             ** eapply assgn_varsIn_monotonic, K1; cbn; intros; lia.
+             ** eapply assgn_varsIn_monotonic, G1; cbn; intros; lia. 
+             ** eapply assgn_varsIn_monotonic, H0'; cbn; intros; lia. 
+          ++ lia.
+      * (*second formula is false*)
+        assert (evalVar (join a2' a) rv2 = false) as He'. 
+        { destruct (evalVar (join a2' a) rv2); [ | easy]. unfold FSAT.satisfies in K3. rewrite He in K3; firstorder. }
+        exists (a2' ++ a1'). split; [ | split].
+        -- rewrite !assgn_varsIn_app. split.
+           ++ eapply assgn_varsIn_monotonic, K1. cbn; intros; lia.
+           ++ eapply assgn_varsIn_monotonic, G1. cbn; intros; lia.
+        -- unfold join, satisfies. rewrite !evalCnf_app_iff. repeat split.
+           ++ rewrite <-app_assoc.  
+             erewrite <- join_extension_cnf_sat; [apply G2 | apply IH1 | apply K1 | cbn; intros; lia]. 
+           ++ enough (evalCnf (join a1' (join a2' a)) N2 = true) as Hee.
+             { rewrite <- Hee. apply evalCnf_assgn_equiv. unfold join; list_equiv. } 
+             erewrite <- join_extension_cnf_sat; [apply K2 | apply IH4 | apply G1 | cbn; intros; lia].
+           ++ apply tseytinAnd_sat. 
+              erewrite evalVar_not_assgn_varsIn_false with (p := fun n => n < b \/ (n >= nf /\ n < nfVar2)). 
+              2: { rewrite <- app_assoc, !assgn_varsIn_app. split; [ | split]. 
+                  - eapply assgn_varsIn_monotonic, K1. cbn; intros; lia.
+                  - eapply assgn_varsIn_monotonic, G1. cbn; intros; lia.
+                  - eapply assgn_varsIn_monotonic, H0'. cbn; intros; lia.
+              } 
+              2: lia. 
+              rewrite <- !app_assoc. 
+              setoid_rewrite evalVar_assgn_equiv with (a' := a1' ++ a2' ++ a) at 2. 2: list_equiv. 
+              setoid_rewrite <- join_extension_var_sat  with (p1 := fun n => n = rv2) at 2.
+              ** unfold join in He'. rewrite He'. firstorder.
+              ** reflexivity. 
+              ** apply G1. 
+              ** cbn; intros; lia.
+       -- unfold FSAT.satisfies. rewrite H0. rewrite evalVar_not_assgn_varsIn_false with (p := fun n => n < b \/ (n >= nf /\ n < nfVar2)); [easy | | ].  
+          ++ unfold join. rewrite !assgn_varsIn_app. split; [ split| ].
+             ** eapply assgn_varsIn_monotonic, K1; cbn; intros; lia.
+             ** eapply assgn_varsIn_monotonic, G1; cbn; intros; lia. 
+             ** eapply assgn_varsIn_monotonic, H0'; cbn; intros; lia. 
+          ++ lia.
+  - clear IH61 IH31. intros H1. unfold satisfies in H0. rewrite !evalCnf_app_iff in H0. destruct H0 as (H2 & H3 & H4).
+    apply tseytinAnd_sat in H4. apply H4 in H1 as (H1 & H1'). 
+    apply IH62 in H3. apply H3 in H1'. 
+    apply IH32 in H2. apply H2 in H1. 
+    now apply evalFormula_and_iff. 
+  - clear IH61 IH31. intros H1. unfold satisfies in H0. rewrite !evalCnf_app_iff in H0. destruct H0 as (H2 & H3 & H4).
+    apply evalFormula_and_iff in H1 as (H5 & H6). 
+    apply tseytinAnd_sat in H4. apply H4. split.
+    + apply (IH32 _ H2), H5. 
+    + apply (IH62 _ H3), H6.
+Qed. 
+
+Lemma or_compat f1 f2 b: 
+  varBound_formula b f1 -> varBound_formula b f2 
+  -> (forall nf nf' v N, nf >= b -> tseytin' nf f1 = (v, N, nf') -> cnf_varsIn (fun n => n < b \/ (n >= nf /\ n < nf')) N /\ v >= nf /\ v < nf' /\ tseytin_formula_repr f1 N v b nf nf')
+  -> (forall nf nf' v N, nf >= b -> tseytin' nf f2 = (v, N, nf') -> cnf_varsIn (fun n => n < b \/ (n >= nf /\ n < nf')) N /\ v >= nf /\ v < nf' /\ tseytin_formula_repr f2 N v b nf nf')
+  -> forall nf nf' v N, nf >= b -> tseytin' nf (f1 ∨ f2) = (v, N, nf') -> cnf_varsIn (fun n => n < b \/ (n >= nf /\ n < nf')) N /\ v >= nf /\ v < nf' /\ tseytin_formula_repr (f1 ∨ f2) N v b nf nf'. 
+Proof. 
+  cbn. intros bound1 bound2 IHf1 IHf2 nf nf' v N H H0. 
+  destruct (tseytin' nf f1) as ((rv1 & N1) & nfVar1) eqn:F1. 
+  destruct (tseytin' nfVar1 f2) as ((rv2 & N2) & nfVar2) eqn:F2. 
+  specialize (IHf1 nf nfVar1 _ _ ltac:(lia) F1) as (IH1 & IH2 & IH2' & (IH31 & IH32)). 
+  specialize (tseytin'_nf_monotonic F1) as H7. 
+  specialize (tseytin'_nf_monotonic F2) as H8.
+  specialize (IHf2 nfVar1 nfVar2 _ _ ltac:(lia) F2) as (IH4 & IH5 & IH5' & (IH61 & IH62)). clear F1 F2.
+  symmetry in H0. inv H0. split; [ | split; [lia | split; [lia | split;[ | split]]]]. 
+  - repeat rewrite cnf_varsIn_app. 
+    repeat split.
+    + eapply cnf_varsIn_monotonic, IH1; cbn; intros. lia. 
+    + eapply cnf_varsIn_monotonic, IH4; cbn; intros; lia. 
+    + eapply cnf_varsIn_monotonic, tseytinOr_cnf_varsIn; cbn; intros; lia.
+  - intros a H0'. clear IH32 IH62. 
+    (*unfold FSAT.satisfies in H0. apply evalFormula_or_iff in H0 as [He | He].*)
+    (*+ apply IH31 in He as (a1' & G1 & G2); [ | apply H0']. *)
+      (*specialize (IH63 a H0') as (a2' & G3 & G4). *)
+      (*exists (nfVar2 :: a'). split.*)
+      (*{ rewrite app_singleton. apply assgn_varsIn_app; split. *)
+        (*- intros v' [-> | []]. lia.*)
+        (*- eapply assgn_varsIn_monotonic, G1. cbn; intros; lia. *)
       (*} *)
-      (*unfold join. cbn. unfold satisfies.*)
-      (*rewrite app_singleton in G2, G4. apply evalCnf_app_iff in G2. apply evalCnf_app_iff in G4. *)
-      (*setoid_rewrite app_singleton at 2. repeat rewrite evalCnf_app_iff; repeat split.*)
-      (** cbn. rewrite Nat.eqb_refl. easy.*)
-      (** destruct G2 as (_ & G2). clear G4. *)
-        (*replace (nfVar2 :: (a2' ++ a1') ++ a) with (join (nfVar2 :: a2') (a1' ++ a)) by (unfold join; firstorder). *)
-        (*eapply (join_extension_cnf_monotonic). apply G2. *)
-      (** destruct G4 as (_ & G4). clear G2. *)
-        (*unfold join in G4. rewrite app_singleton.*)
-        (*enough (evalCnf ([nfVar2] ++ a1' ++ a2' ++ a) N2 = true). *)
-        (*{ rewrite <- H. eapply evalCnf_assgn_equiv. rewrite <- app_assoc. *)
-          (*split; intros x; rewrite !in_app_iff in *; intros Hx; destruct_or Hx; eauto. *)
-        (*} *)
-        (*replace ([nfVar2] ++ a1' ++ a2' ++a) with (join (nfVar2 :: a1') (a2' ++ a)) by (unfold join; firstorder).*)
-        (*eapply (join_extension_cnf_monotonic). apply G4. *)
-      (** apply tseytinAnd_sat. split; [intros _ | intros _; cbn; rewrite Nat.eqb_refl; easy]. *)
-        (*destruct G2 as (G2 & _). destruct G4 as (G4 & _). *)
-        (*cbn in G2, G4. rewrite Bool.eqb_true_iff in G2. rewrite Bool.eqb_true_iff in G4.*)
-        (*split; eapply evalVar_monotonic. *)
-        (*2: apply G2. 3: apply G4. *)
-        (*all: unfold join; rewrite <- app_assoc, app_singleton; intros x; rewrite !in_app_iff; intros Hx; destruct_or Hx; eauto. *)
-    (*+ clear IH61 IH31. *)
-      (*cbn. apply evalFormula_and_iff. split.*)
-      (** enough (FSAT.satisfies (restrict a (formula_maxVar f1)) f1). *)
-        (*{ apply restrict_formula_equisat. 1: { eapply varBound_formula_monotonic; [ | apply formula_bound_varBound]. lia. }*)
-          (*apply restrict_formula_equisat in H0; [easy | apply formula_bound_varBound]. *)
-        (*} *)
-        (*eapply IH32. rewrite app_singleton in H. unfold satisfies in H. rewrite !evalCnf_app_iff in H.*)
-        (*destruct H as (X1 & X2 & _ & X4). *)
-        (*cbn in X1. apply eqb_prop in X1.*)
-        (*apply tseytinAnd_sat in X4. apply X4 in X1 as (X1 & _).*)
-        (*unfold satisfies. rewrite app_singleton, evalCnf_app_iff. *)
-        (*split; [ cbn; now rewrite X1 | apply X2]. *)
-      (** enough (FSAT.satisfies (restrict a (formula_maxVar f2)) f2). *)
-        (*{ apply restrict_formula_equisat. 1: { eapply varBound_formula_monotonic; [ | apply formula_bound_varBound]. lia. }*)
-          (*apply restrict_formula_equisat in H0; [easy | apply formula_bound_varBound]. *)
-        (*} *)
-        (*eapply IH62. rewrite app_singleton in H. unfold satisfies in H. rewrite !evalCnf_app_iff in H.*)
-        (*destruct H as (X1 & _ & X3 & X4). *)
-        (*cbn in X1. apply eqb_prop in X1.*)
-        (*apply tseytinAnd_sat in X4. apply X4 in X1 as (_ & X1).*)
-        (*unfold satisfies. rewrite app_singleton, evalCnf_app_iff. *)
-        (*split; [ cbn; now rewrite X1 | apply X3]. *)
-(*Qed.*)
+      (*unfold join. cbn. rewrite app_singleton. setoid_rewrite app_singleton at 3. unfold satisfies. rewrite !evalCnf_app_iff.  *)
+      (*rewrite app_singleton in G2. unfold satisfies in G2. rewrite evalCnf_app_iff in G2. destruct G2 as [G2 G2'].*)
+      (*repeat split.*)
+      (** cbn. now rewrite Nat.eqb_refl.*)
+      (** replace ([nfVar2] ++ a' ++a) with (join [nfVar2] (a' ++a)) by (unfold join; easy).*)
+        (*rewrite <- join_extension_cnf_sat with (p2 := fun n => n = nfVar2).*)
+        (*-- apply G2'.*)
+        (*-- apply IH1. *)
+        (*-- intros v' [-> | []]; cbn; lia.*)
+        (*-- cbn; intros; lia.*)
+      (** replace ([nfVar2] ++ a' ++ a) with (join ([nfVar2] ++ a') a) by (unfold join; firstorder).*)
+        (*rewrite <- join_extension_cnf_sat with (p2 := fun n => n = nfVar2 \/ (n >= nf /\ n < nfVar1)).*)
+        (*-- apply IH63, H0'. *)
+        (*-- apply IH4.*)
+        (*-- apply assgn_varsIn_app. split; [intros v' [-> | []]; cbn; lia | ].*)
+           (*eapply assgn_varsIn_monotonic, G1; cbn; intros; lia.*)
+        (*-- cbn; intros; lia.*)
+      (** apply tseytinOr_sat. cbn in G2. apply eqb_prop in G2.*)
+        (*split; [ intros _ | intros _; cbn; now rewrite Nat.eqb_refl]. left. *)
+        (*replace ([nfVar2 ] ++ a' ++ a) with (join [nfVar2] (join a' a)) by (unfold join; firstorder). *)
+        (*erewrite <- join_extension_var_sat with (p1 := fun n => n = rv1) (p2 := fun n => n = nfVar2). *)
+        (*-- apply G2.*)
+        (*-- easy.*)
+        (*-- intros v' [-> | []]; cbn; lia.*)
+        (*-- intros; cbn; lia.*)
+    (*+ apply IH61 in He as (a' & G1 & G2); [ | apply H0']. exists (nfVar2 :: a'). split.*)
+      (*{ rewrite app_singleton. apply assgn_varsIn_app; split. *)
+        (*- intros v' [-> | []]. lia.*)
+        (*- eapply assgn_varsIn_monotonic, G1. cbn; intros; lia. *)
+      (*} *)
+      (*unfold join. cbn. rewrite app_singleton. setoid_rewrite app_singleton at 3. unfold satisfies. rewrite !evalCnf_app_iff.  *)
+      (*rewrite app_singleton in G2. unfold satisfies in G2. rewrite evalCnf_app_iff in G2. destruct G2 as [G2 G2'].*)
+      (*repeat split.*)
+      (** cbn. now rewrite Nat.eqb_refl.*)
+      (** replace ([nfVar2] ++ a' ++ a) with (join ([nfVar2] ++ a') a) by (unfold join; firstorder).*)
+        (*rewrite <- join_extension_cnf_sat with (p2 := fun n => n = nfVar2 \/ (n >= nfVar1 /\ n < nfVar2)).*)
+        (*-- apply IH33, H0'. *)
+        (*-- apply IH1.*)
+        (*-- apply assgn_varsIn_app. split; [intros v' [-> | []]; cbn; lia | ].*)
+           (*eapply assgn_varsIn_monotonic, G1; cbn; intros; lia.*)
+        (*-- cbn; intros; lia.*)
+      (** replace ([nfVar2] ++ a' ++a) with (join [nfVar2] (a' ++a)) by (unfold join; easy).*)
+        (*rewrite <- join_extension_cnf_sat with (p2 := fun n => n = nfVar2).*)
+        (*-- apply G2'.*)
+        (*-- apply IH4. *)
+        (*-- intros v' [-> | []]; cbn; lia.*)
+        (*-- cbn; intros; lia.*)
+      (** apply tseytinOr_sat. cbn in G2. apply eqb_prop in G2.*)
+        (*split; [ intros _ | intros _; cbn; now rewrite Nat.eqb_refl]. right.*)
+        (*replace ([nfVar2 ] ++ a' ++ a) with (join [nfVar2] (join a' a)) by (unfold join; firstorder). *)
+        (*erewrite <- join_extension_var_sat with (p1 := fun n => n = rv2) (p2 := fun n => n = nfVar2). *)
+        (*-- apply G2.*)
+        (*-- easy.*)
+        (*-- intros v' [-> | []]; cbn; lia.*)
+        (*-- intros; cbn; lia.*)
+  (*- clear IH61 IH31 IH63 IH33. intros a H0.*)
+    (*cbn. apply evalFormula_or_iff.*)
+    (*rewrite app_singleton in H0. unfold satisfies in H0. rewrite !evalCnf_app_iff in H0. *)
+    (*destruct H0 as (X1 & X2 & X3 & X4).*)
+    (*cbn in X1. apply eqb_prop in X1.*)
+    (*apply tseytinOr_sat in X4. apply X4 in X1 as [X1 | X1].*)
+    (** left. apply IH32. *)
+      (*unfold satisfies. rewrite app_singleton, evalCnf_app_iff. *)
+      (*split; [ cbn; now rewrite X1 | apply X2]. *)
+    (** right. apply IH62. *)
+      (*unfold satisfies. rewrite app_singleton, evalCnf_app_iff. *)
+      (*split; [ cbn; now rewrite X1 | apply X3]. *)
+  (*- clear IH61 IH31 IH62 IH32. intros a He. unfold satisfies. rewrite !evalCnf_app_iff. *)
+    (*split; [apply IH33, He | split; [ apply IH63, He | ]].*)
+    (*apply tseytinOr_sat. erewrite !evalVar_not_assgn_varsIn_false. 1: tauto.*)
+    (*1, 3, 5: apply He. all: cbn; lia. *)
+(*Qed. *)
 Admitted. 
 
-(*Lemma or_compat f1 f2: *)
-  (*(forall nf nf' v N, varBound_formula nf f1 -> tseytin' nf f1 = (v, N, nf') -> varBound_cnf nf' N /\ v < nf' /\ tseytin_formula_repr f1 N v nf)*)
-  (*-> (forall nf nf' v N, varBound_formula nf f2 -> tseytin' nf f2 = (v, N, nf') -> varBound_cnf nf' N /\ v < nf' /\ tseytin_formula_repr f2 N v nf)*)
-  (*-> forall nf nf' v N, varBound_formula nf (f1 ∨ f2) -> tseytin' nf (f1 ∨ f2) = (v, N, nf') -> varBound_cnf nf' N /\ v < nf' /\ tseytin_formula_repr (f1 ∨ f2) N v nf. *)
-(*Proof. *)
- 
-(*Admitted.  *)
+Lemma not_compat f b : 
+  varBound_formula b f 
+  -> (forall nf nf' v N, nf >= b -> tseytin' nf f = (v, N, nf') -> cnf_varsIn (fun n => n < b \/ (n >= nf /\ n < nf')) N /\ v >= nf /\ v < nf' /\ tseytin_formula_repr f N v b nf nf')
+  -> forall nf nf' v N, nf >= b -> tseytin' nf (¬ f) = (v, N, nf') -> cnf_varsIn (fun n => n < b \/ (n >= nf /\ n < nf')) N /\ v >= nf /\ v < nf' /\ tseytin_formula_repr (¬ f) N v b nf nf'.
+Proof. 
+  cbn. intros bound IHf nf nf' v N H H0.  
+  destruct (tseytin' nf f) as ((rv & N') & nfVar') eqn:F1. 
+  specialize (IHf nf nfVar' _ _ ltac:(lia) F1) as (IH1 & IH2 & IH2' & (IH31 & IH32)). 
+  specialize (tseytin'_nf_monotonic F1) as H1. 
+  symmetry in H0. inv H0. split; [ | split; [lia | split; [lia | split]]]. 
+  - rewrite cnf_varsIn_app. split.
+    + eapply cnf_varsIn_monotonic, IH1. cbn; intros; lia.
+    + eapply cnf_varsIn_monotonic, tseytinNot_cnf_varsIn. cbn; intros; lia.
+  - clear IH32. intros a H2. 
+    specialize (IH31 a H2) as (a1' & G1 & G2 & G3).
+    unfold FSAT.satisfies in *. cbn. destruct (evalFormula a f) eqn:H0; cbn.
+    + exists a1'. specialize (proj1 G3 eq_refl) as G3'. clear G3.
+      split.
+      * eapply assgn_varsIn_monotonic, G1. cbn; intros; lia.
+      * assert (evalVar (join a1' a) nfVar' = false) as He. 
+        { eapply evalVar_not_assgn_varsIn_false with (p := fun n => n < b \/ (n >= nf /\ n < nfVar')).
+          2: cbn; lia.
+          apply assgn_varsIn_app; split; eapply assgn_varsIn_monotonic; eauto; cbn; intros; lia.
+        } 
+        split; [ | rewrite He; tauto].
+        apply evalCnf_app_iff. split; [ apply G2 | ].
+        apply tseytinNot_sat. rewrite G3'. now rewrite He. 
+    + exists ([nfVar'] ++ a1'). assert (evalVar (join a1' a) rv = false) as G3'.
+      { destruct evalVar; [ firstorder | easy]. } clear G3.
+      split; [ | split].
+      * apply assgn_varsIn_app; split; [intros v' [-> | []]; cbn; intros; lia | ].
+        eapply assgn_varsIn_monotonic, G1; cbn; intros; lia.
+      * apply evalCnf_app_iff; split.
+        -- replace (join ([nfVar'] ++ a1') a) with (join [nfVar'] (join a1' a)) by (unfold join; firstorder).
+           erewrite <- join_extension_cnf_sat with (p2 := fun n => n = nfVar'). 
+           ++ apply G2.
+           ++ apply IH1. 
+           ++ intros v' [-> | []]; cbn; lia.
+           ++ cbn; intros; lia.
+        -- apply tseytinNot_sat. split; [ intros _| cbn; intros _; now rewrite Nat.eqb_refl].
+           replace (join ([nfVar'] ++ a1') a) with (join [nfVar'] (join a1' a)) by (unfold join; firstorder).
+           erewrite <- join_extension_var_sat with (p1 := fun n => n = rv) (p2 := fun n => n = nfVar'). 
+           ++ now rewrite G3'.
+           ++ easy.
+           ++ intros v' [-> | []]; cbn; lia.
+           ++ cbn; intros; lia.
+      * cbn; rewrite Nat.eqb_refl; firstorder.
+  - intros a H0. apply evalCnf_app_iff in H0 as (H0 & H0'). 
+    specialize (IH32 a H0). apply tseytinNot_sat in H0'. 
+    split.
+    + intros H2. apply H0' in H2. 
+      enough (not (FSAT.satisfies (restrict a b) f)) as Ha.
+      { unfold FSAT.satisfies in *. apply evalFormula_not_iff, Ha. } 
+      now rewrite <- IH32.
+    + intros H2. apply H0'. rewrite IH32. now apply evalFormula_not_iff in H2.
+Qed.
 
-(*Lemma not_compat f: *)
-  (*(forall nf nf' v N, varBound_formula nf f -> tseytin' nf f = (v, N, nf') -> varBound_cnf nf' N /\ v < nf' /\ tseytin_formula_repr f N v nf)*)
-  (*-> forall nf nf' v N, varBound_formula nf (¬ f) -> tseytin' nf (¬ f) = (v, N, nf') -> varBound_cnf nf' N /\ v < nf' /\ tseytin_formula_repr (¬ f) N v nf. *)
-(*Proof. *)
- 
-(*Admitted. *)
-       
-Lemma tseytin'_repr b f nf v N nf' : varBound_formula b f -> nf >= b -> tseytin' nf f = (v, N, nf') -> cnf_varsIn (fun n => n < b \/ (n >= nf /\ n < nf')) N /\ v < nf' /\ tseytin_formula_repr f N v nf. 
+Lemma tseytin'_repr b f nf v N nf' : varBound_formula b f -> nf >= b -> tseytin' nf f = (v, N, nf') -> cnf_varsIn (fun n => n < b \/ (n >= nf /\ n < nf')) N /\ v >= nf /\ v < nf' /\ tseytin_formula_repr f N v b nf nf'. 
 Proof. 
   intros H. revert nf nf' v N. induction f; intros. 
   - inv H. cbn in H1. inv H1. split. 
     1 : { intros v'. intros (c & [<- | []] & (l & [<- | []] & H)). destruct H as (? & H). inv H. lia. } 
-    split; [ lia | split; intros]. 
-    + exists [v]; cbn. split. 
+    split; [ lia | split; [lia | split]]. 
+    + intros a H. exists [v]; cbn. split; [ | split]. 
       * intros v' [-> | []]. lia.
-      *  unfold satisfies. do 2 (cbn; rewrite Nat.eqb_refl). easy. 
-    + easy.
-  - inv H. split. 
-    1: { cbn in H1. inv H1. intros v'. intros (c & [] & H). }
-    inv H1. split; [ lia | split].
-    + intros a H2. unfold FSAT.satisfies in H2. apply evalFormula_prim_iff in H2. unfold satisfies. 
-      exists []. cbn. split; [easy | ].
-      apply Bool.eqb_true_iff. now apply evalVar_in_iff. 
-    + intros a H1. unfold satisfies in H1. cbn in H1. apply Bool.eqb_prop in H1. apply evalVar_in_iff in H1. 
-      apply restrict_formula_equisat. 1: apply formula_bound_varBound.
-      apply evalFormula_prim_iff, H1.
+      * unfold satisfies. cbn. now rewrite Nat.eqb_refl. 
+      * rewrite Nat.eqb_refl. cbn. unfold FSAT.satisfies. easy.
+    + intros a H. unfold satisfies in H. cbn in H. apply eqb_prop in H. unfold FSAT.satisfies; easy.
+  - inv H. cbn in H1. inv H1. split. 
+    1: { eapply cnf_varsIn_monotonic, tseytinEquiv_cnf_varsIn. cbn; intros n0; lia. }
+    split; [ lia | split; [lia | split ]].
+    + intros a H1. unfold FSAT.satisfies. 
+      exists (if evalVar a n then [v] else []). 
+      split; [ | split].
+      * destruct evalVar; [ intros v' [-> | []]; cbn; lia | easy].
+      * apply tseytinEquiv_sat. rewrite !evalVar_in_iff. 
+        destruct (evalVar a n) eqn:H2.
+        -- cbn. apply evalVar_in_iff in H2. easy.
+        -- cbn. assert (not (evalVar a n = true)) as H by congruence. rewrite evalVar_in_iff in H. 
+           enough (not (v el a)) by tauto. intros Hel. specialize (H1 v Hel). cbn in H1; lia.
+      * unfold evalFormula. destruct evalVar.
+        -- split; [intros _; cbn; rewrite Nat.eqb_refl; easy | easy].
+        -- split; [ congruence | ]. intros H%evalVar_in_iff. cbn in H. apply H1 in H. lia.
+    + intros a H. apply tseytinEquiv_sat in H. rewrite <- H.
+      unfold FSAT.satisfies. cbn. unfold evalVar. rewrite !list_in_decb_iff.
+      2, 3: symmetry; apply Nat.eqb_eq. unfold restrict; rewrite in_filter_iff.
+      rewrite Nat.ltb_lt. tauto.
   - inv H. apply (varBound_formula_monotonic H6) in H4. apply (varBound_formula_monotonic H7) in H5. 
     now apply (and_compat H4 H5  (IHf1 H4) (IHf2 H5)).
-  (*- now apply (or_compat IHf1 IHf2).*)
-  (*- now apply (not_compat IHf).*)
-Admitted. 
-
-Proposition tseytin_formula_repr_s f N v nf: tseytin_formula_repr f N v nf -> formula_repr f N v. 
-Proof. 
-  intros [H1 H2]. split.
-  - intros (a & H). apply H1 in H as (a' & _ & H). exists (join a' a). apply H. 
-  - intros (a & H). apply H2 in H. exists (restrict a (formula_maxVar f)). apply H. 
+  - inv H. apply (varBound_formula_monotonic H6) in H4. apply (varBound_formula_monotonic H7) in H5. 
+    now apply (or_compat H4 H5  (IHf1 H4) (IHf2 H5)).
+  - inv H. now apply (not_compat H3 (IHf H3)). 
 Qed. 
 
-Lemma tseytin_repr f v N : tseytin f = (v, N) -> formula_repr f N v. 
+Proposition assgn_varsIn_restrict a b: assgn_varsIn (fun n => n < b) (restrict a b). 
+Proof. 
+  intros v. unfold restrict. rewrite in_filter_iff. intros (_ & H%Nat.ltb_lt). apply H.
+Qed.
+
+Proposition tseytin_formula_repr_s f N v nf nf': tseytin_formula_repr f N v (formula_maxVar f) nf nf' -> formula_repr f N v. 
+Proof. 
+  intros [H1 H2]. split.
+  - intros (a & H). eapply restrict_formula_equisat in H. 2: apply formula_bound_varBound.
+    edestruct (H1 (restrict a (formula_maxVar f))) as (a' & _ & F2 & F3).
+    { apply assgn_varsIn_restrict. }
+    apply F3 in H. exists (join a' (restrict a (formula_maxVar f))). 
+    rewrite app_singleton. apply evalCnf_app_iff. split.
+    + cbn. rewrite H. easy. 
+    + apply F2. 
+  - intros (a & H). 
+    rewrite app_singleton in H. apply evalCnf_app_iff in H as (H3 & H4). 
+    apply H2 in H4. cbn in H3. apply eqb_prop in H3. apply H4 in H3.
+    exists (restrict a (formula_maxVar f)). apply H3. 
+Qed. 
+
+Theorem tseytin_repr f v N : tseytin f = (v, N) -> formula_repr f N v. 
 Proof. 
   unfold tseytin. destruct tseytin' as ((repVar & N1) & nfvar') eqn:H1.
   intros H; inv H. 
-  specialize (tseytin'_repr). 
-  eapply tseytin'_repr; [ | apply H1].
-  apply formula_bound_varBound.
+  eapply tseytin'_repr in H1. 
+  - eapply tseytin_formula_repr_s, H1. 
+  - apply formula_bound_varBound. 
+  - lia.
 Qed.
-  
 
+Definition reduction f := let (v, N) := tseytin f in [(true, v)] :: N. 
 
+Lemma FSAT_to_SAT f : FSAT f <-> SAT (reduction f). 
+Proof. 
+  unfold reduction. destruct (tseytin f) eqn:H1. 
+  apply tseytin_repr in H1 as (H1 & H2). tauto. 
+Qed.  
